Cslib/Computability/Machines/MultiTapeTuring/GraphReachability.lean
@@ -8,13 +8,17 @@ module
 
 public import Cslib.Computability.Machines.MultiTapeTuring.Basic
 public import Cslib.Computability.Machines.MultiTapeTuring.ListEncoding
-public import Cslib.Computability.Machines.MultiTapeTuring.HeadStats
+public import Cslib.Computability.Machines.MultiTapeTuring.IteCombinator
+public import Cslib.Computability.Machines.MultiTapeTuring.SequentialCombinator
+public import Cslib.Computability.Machines.MultiTapeTuring.EqualRoutine
+public import Cslib.Computability.Machines.MultiTapeTuring.PushRoutine
+public import Cslib.Computability.Machines.MultiTapeTuring.PopRoutine
+public import Cslib.Computability.Machines.MultiTapeTuring.DuplicateRoutine
 
--- TODO create a "common file"
-import Cslib.Computability.Machines.SingleTapeTuring.Basic
 
 namespace Turing
 
+namespace Routines
 
 -- This is an attempt at proving Savitch's theorem. We start by stating a generic
 -- space-efficient graph reachability algorithm.
@@ -35,62 +39,159 @@ def reachable(a, b, t, r):
 Until we have a generic mechanism for recursion, let's translate this into a program that
 uses "goto", and every variable is a stack:
 
-def reachable(a, b, t, r):
-  terminate = 0
+def reachable(a, b, t, edge):
   result = 0
   initial_t = t
-  section = [:terminate, :fun_start]
-  while !terminate:
-    match section.pop()
+  pc = [:fun_start]
+  while !pc.is_empty():
+    match pc.pop()
     | :fun_start =>
       if t = 0:
-        result = r(a, b)
-        section.push(:fun_return)
+        result = edge(a, b)
       else:
         c.push(0)
-        section.push(:loop_start)
+        pc.push(:loop_start)
     | :loop_start =>
       if c.top() = num_vertices:
         c.pop()
         result = 0
-        section.push(:fun_return)
       else:
         a.push(a.top())
         b.push(c.top())
-        t.push(t.top() - 1)
-        section.push(:after_first_rec)
-        section.push(:fun_start)
+        t = t - 1
+        pc.push(:after_first_rec)
+        pc.push(:fun_start)
     | :after_first_rec =>
+        a.pop()
+        b.pop()
+        t = t + 1
         if result == 1:
           a.push(c.top())
           b.push(b.top())
-          t.push(t.top() - 1)
-          section.push(:after_second_rec)
-          section.push(0)
+          t = t - 1
+          pc.push(:after_second_rec)
+          pc.push(:fun_start)
         else:
           result = 0
-          section.push(:loop_continue)
+          pc.push(:loop_continue)
     | :after_second_rec =>
+        a.pop()
+        b.pop()
+        t = t + 1
         if result == 1:
           c.pop()
-          section.push(:fun_return)
         else:
-          section.push(:loop_continue)
+          pc.push(:loop_continue)
     | :loop_continue =>
         c.push(c.top() + 1)
-        section.push(:loop_start)
-    | :fun_return =>
-      a.pop()
-      b.pop()
-      t.pop()
-    | :terminate =>
-      terminate = 1
+        pc.push(:loop_start)
   -- cleanup
-  terminate.pop()
   initial_t.pop()
-
-
+  t.pop()
+  a.pop()
+  b.pop()
 -/
 
+def tapeCount := 20
 
+lemma tape_count_eq : tapeCount = 20 := rfl
+
+def a : Fin tapeCount := ⟨3, sorry⟩
+def b : Fin tapeCount := ⟨4, sorry⟩
+def t : Fin tapeCount := ⟨5, sorry⟩
+def result : Fin tapeCount := ⟨6, sorry⟩
+def initialT : Fin tapeCount := ⟨7, sorry⟩
+def pc : Fin tapeCount := ⟨8, sorry⟩
+def c : Fin tapeCount := ⟨9, sorry⟩
+def mainAux : Fin tapeCount := ⟨10, sorry⟩
+
+def l_funStart := dya 1
+def l_loopStart := dya 2
+
+-- if t = 0:
+--   result = edge(a, b)
+-- else:
+--   c.push(0)
+--   pc.push(:loop_start)
+
+def funStart (edge : MultiTapeTM tapeCount (WithSep OneTwo)) :=
+  ite t (push c [] <;> push pc l_loopStart) edge
+
+@[simp]
+lemma funStart_eval_list
+  (tapes : Fin tapeCount → List (List OneTwo))
+  (edge : MultiTapeTM tapeCount (WithSep OneTwo)) :
+  (funStart edge).eval_list tapes =
+    if (tapes t).headD [] = [] then
+      (edge.eval_list tapes)
+    else
+      .some (Function.update (Function.update tapes c ([] :: (tapes c)))
+        pc (l_loopStart :: (tapes pc))) := by
+  have : pc ≠ c := by decide
+  simp [funStart]
+  grind
+
+def infiniteLoop {α : Type} {k : ℕ} : MultiTapeTM k (WithSep α) := sorry
+
+public def eqLit {k : ℕ}
+  (q : Fin (k + 3))
+  (w : List OneTwo)
+  (s : Fin (k + 3))
+  (aux : Fin (k + 3) := ⟨k + 2, by omega⟩)
+  (h_inj : [q, aux, s].get.Injective := by intro x y; grind) :
+  MultiTapeTM (k + 3) (WithSep OneTwo) :=
+    push aux w <;> eq q aux s h_inj <;> pop aux
+
+public theorem eqLit_eval_list {k : ℕ} {q s aux : Fin (k + 3)} {w : List OneTwo}
+  {h_inj : [q, aux, s].get.Injective}
+  {tapes : Fin (k + 3) → List (List OneTwo)} :
+  (eqLit q w s aux h_inj).eval_list tapes =
+    .some (Function.update tapes s (
+      (if (tapes q).headD [] = w then
+        [.one]
+      else
+        []) :: (tapes s))) := by
+  simp [eqLit, eq_eval_list h_inj]
+  have h_neq : aux ≠ s := Function.Injective.ne h_inj (a₁ := 1) (a₂ := 2) (by grind)
+  have h_neq : q ≠ aux := Function.Injective.ne h_inj (a₁ := 0) (a₂ := 1) (by grind)
+  grind
+
+-- | :loop_start =>
+-- if c.top() = num_vertices:
+--   c.pop()
+--   result = 0
+-- else:
+--   a.push(a.top())
+--   b.push(c.top())
+--   t = t - 1
+--   pc.push(:after_first_rec)
+--   pc.push(:fun_start)
+
+def loopStart (maxConfig : List OneTwo) :=
+  eqLit c maxConfig mainAux <;>
+    ite mainAux
+      (pop mainAux <;> pop c <;> push result [])
+      (duplicate a <;> copy c b <;> dec t <;> push pc l_funStart <;> push pc l_loopStart)
+
+public def matchCombine {k : ℕ}
+  (i : Fin (k + 3)) (aux : Fin (k + 3)) (h_inj : [i, aux, aux + 1].get.Injective)
+  (branches : List ((List OneTwo) × (MultiTapeTM (k + 3) (WithSep OneTwo)))) :
+  MultiTapeTM (k + 3) (WithSep OneTwo) :=
+  match branches with
+  | [] => infiniteLoop
+  | (w, tm) :: branches =>
+      eqLit i w aux (aux + 1) (h_inj := by sorry /- use swap on h_inj? -/) <;>
+        ite aux (pop aux <;> tm) (pop aux <;> matchCombine i aux (by intro x y; grind) branches)
+
+def innerLoop (edge : MultiTapeTM tapeCount (WithSep OneTwo)) :
+    MultiTapeTM tapeCount (WithSep OneTwo) :=
+  matchCombine pc mainAux (by decide)
+  [ (l_funStart, funStart edge),
+    (l_loopStart, loop 1, infiniteLoop) ]
+
+
+
+theorem reachable
+
+end Routines
 end Turing
