Cslib/Computability/Machines/MultiTapeTuring/DecRoutine.lean
@@ -1,0 +1,101 @@
+/-
+Copyright (c) 2026 Christian Reitwiessner. All rights reserved.
+Released under Apache 2.0 license as described in the file LICENSE.
+Authors: Christian Reitwiessner
+-/
+
+module
+
+public import Cslib.Computability.Machines.MultiTapeTuring.Basic
+public import Cslib.Computability.Machines.MultiTapeTuring.ListEncoding
+public import Cslib.Computability.Machines.MultiTapeTuring.WithTapes
+public import Cslib.Computability.Machines.MultiTapeTuring.CopyRoutine
+public import Cslib.Computability.Machines.MultiTapeTuring.SuccRoutine
+public import Cslib.Computability.Machines.MultiTapeTuring.PushRoutine
+public import Cslib.Computability.Machines.MultiTapeTuring.PopRoutine
+public import Cslib.Computability.Machines.MultiTapeTuring.SequentialCombinator
+public import Cslib.Computability.Machines.MultiTapeTuring.LoopCombinator
+
+namespace Turing
+
+namespace Routines
+
+def dec₀ : MultiTapeTM 6 (WithSep OneTwo) :=
+  push 1 [] <;> push 2 [] <;>
+  loop 0 (h_i := by decide) (pop 2 <;> copy 1 2 <;> succ 1) <;>
+  pop 0 <;>
+  copy 2 0 <;>
+  pop 2 <;>
+  pop 1
+
+@[simp]
+lemma inner_eval_list {tapes : Fin 3 → List (List OneTwo)} :
+  (pop 2 <;> copy 1 2 <;> succ 1).eval_list tapes = .some (
+    (if h : tapes 1 = [] then Function.update tapes 2 ((tapes 1).head?.getD [] :: (tapes 2).tail)
+  else
+    Function.update (Function.update tapes 2 ((tapes 1).head?.getD [] :: (tapes 2).tail)) 1
+      (dya (dya_inv ((tapes 1).headD []) + 1) :: (tapes 1).tail))) := by
+  simp
+  grind
+
+@[simp]
+lemma inner_eval_iter {r : ℕ} {tapes : Fin 3 → List (List OneTwo)} :
+  (Part.bind · (pop 2 <;> copy 1 2 <;> succ 1).eval_list)^[r] (.some tapes) = Part.some (
+    if r = 0 then
+      tapes
+    else if tapes 1 = [] then
+      Function.update tapes 2 ([] :: (tapes 2).tail)
+    else
+      Function.update (Function.update tapes
+        2 ((dya ((dya_inv ((tapes 1).headD [])) + (r - 1))) :: (tapes 2).tail))
+        1 ((dya ((dya_inv ((tapes 1).headD [])) + r)) :: (tapes 1).tail)) := by
+  induction r with
+  | zero => simp
+  | succ r ih =>
+    rw [Function.iterate_succ_apply']
+    simp [ih, inner_eval_list, -copy_eval_list, -succ_eval_list, -pop_eval_list, -MultiTapeTM.seq_eval_list]
+    by_cases h_tape1_empty : tapes 1 = []
+    · simp [h_tape1_empty]
+      by_cases h : r = 0
+      · simp [h]; grind
+      · simp [h]; grind
+    · simp [h_tape1_empty]
+      by_cases h : r = 0
+      · simp [h, h_tape1_empty]
+      · simp [h]; grind
+
+@[simp, grind =]
+lemma dec₀_eval_list {tapes : Fin 6 → List (List OneTwo)} :
+  dec₀.eval_list tapes = .some (Function.update tapes 0
+    ((dya ((dya_inv ((tapes 0).headD [])) - 1)) :: (tapes 0).tail)) := by
+  simp [dec₀]
+  grind
+
+/--
+A Turing machine that decrements the dyadic value at the head of tape `i`.
+If the value is zero already, keeps it at zero. If the tape is empty, pushes zero.
+-/
+public def dec {k : ℕ} (i : Fin (k + 3))
+  (aux : Fin (k + 3) := ⟨k, by omega⟩)
+  (h_inj : [i, aux, aux + 1].get.Injective := by intro x y; grind) :
+  MultiTapeTM (k + 6) (WithSep OneTwo) :=
+  push ⟨aux, by omega⟩ [] <;> push ⟨aux + 1, by omega⟩ [] <;>
+  loop i (h_i := by omega) (copy aux (aux + 1) (by sorry) <;> succ aux) <;>
+  pop ⟨i, by omega⟩ <;>
+  copy ⟨aux + 1, by omega⟩ ⟨i, by omega⟩ (by sorry) <;>
+  pop ⟨aux + 1, by omega⟩ <;>
+  pop ⟨aux, by omega⟩
+
+@[simp, grind =]
+public theorem duplicate_eval_list {k : ℕ} {i : Fin k.succ}
+  (aux : Fin k.succ := ⟨k, by omega⟩)
+  (h_inj : [i, aux].get.Injective)
+  {tapes : Fin k.succ → List (List OneTwo)} :
+  (duplicate i aux h_inj).eval_list tapes = Part.some (Function.update tapes i
+    (((tapes i).headD []) :: (tapes i))) := by
+  simp [duplicate]
+  grind
+
+end Routines
+
+end Turing
